nemui.

VeriSkel/Compiler.v
@@ -7,7 +7,7 @@ Require Import LibTactics.
 Require Import Psatz.
 Require Import Monad.
 Require Import MyEnv.
-Require Import SimplSkel.
+Require Import TypedTerm.
 Require Import MyMSets.
 
 Open Scope string_scope.
@@ -41,32 +41,30 @@ Module Sx := Syntax.
 
 Section compiler.
   (* environment of variables of array in the generated code *)
-  Variable avarenv : Env varA (var * list var) _.
-
+  (* Variable avarenv : Env nat (var * list var) _. *)
+  Variable avarenv : list (var * list var).
 
   Fixpoint string_of_ty ty : string :=
     match ty with
-    | Sx.TBool => "Bool"
-    | Sx.TZ => "Z"
-    | Sx.TTup ls => "(" ++ fold_right (fun x y => string_of_ty x ++ y) ")" ls
+    | Skel.TBool => "Bool"
+    | Skel.TZ => "Z"
+    | Skel.TTup t1 t2 => "(" ++ string_of_ty t1 ++ ", " ++ string_of_ty t2 ++ ")"
     end%string.
 
   Fixpoint len_of_ty ty : nat :=
     match ty with
-    | Sx.TBool | Sx.TZ => 1
-    | Sx.TTup ls => fold_right (fun x y => len_of_ty x + y) 0 ls
+    | Skel.TBool | Skel.TZ => 1
+    | Skel.TTup t1 t2 => len_of_ty t1 + len_of_ty t2
     end.
   
   Definition len_until_i tys i : nat :=
     fold_right (fun ty n => len_of_ty ty + n) 0 (firstn i tys).
   
-  Definition len_at_i (tys : list Sx.Typ) i : nat :=
-    len_of_ty (nth i tys Sx.TZ).
+  Definition len_at_i (tys : list Skel.Typ) i : nat :=
+    len_of_ty (nth i tys Skel.TZ).
   
   Import Lang.
   Open Scope string_scope.
-
-  Notation SVEnv := (Env varE (list var) _).
 
   Definition str_of_pnat n m :=
     ("l" ++ S.nat_to_string n ++ "_" ++ S.nat_to_string m).
@@ -132,36 +130,51 @@ Section compiler.
     eapply S.string_inj2; eauto.
   Qed.
 
-  Definition compile_op (op : Sx.SOp) e1 e2 : (cmd * list exp) :=
+  Definition compile_op {t1 t2 t3 : Skel.Typ} (op : Skel.BinOp t1 t2 t3) e1 e2 : (cmd * list exp) :=
     match op with
-    | Sx.Eplus => (Cskip, Lang.Eplus e1 e2 :: nil)
-    | Sx.Emult => (Cskip, Lang.Emult e1 e2 :: nil)
-    | Sx.Emin => (Cskip, Lang.Emin e1 e2 :: nil)
-    | Sx.BEq => (Cskip, Lang.Eeq e1 e2 :: nil)
-    | Sx.Blt => (Cskip, Lang.Elt e1 e2 :: nil)
+    | Skel.Eplus => (Cskip, Lang.Eplus e1 e2 :: nil)
+    | Skel.Emult => (Cskip, Lang.Emult e1 e2 :: nil)
+    | Skel.Emin => (Cskip, Lang.Emin e1 e2 :: nil)
+    | Skel.BEq => (Cskip, Lang.Eeq e1 e2 :: nil)
+    | Skel.Blt => (Cskip, Lang.Elt e1 e2 :: nil)
     end.
 
-  Fixpoint ctyps_of_typ (ty : Sx.Typ) :=
+  Fixpoint ctyps_of_typ (ty : Skel.Typ) :=
     match ty with
-    | Sx.TBool => Int :: nil
-    | Sx.TZ => Int :: nil
-    | Sx.TTup ts => fold_right (fun ty acc => (ctyps_of_typ ty ++ acc)%list) nil ts
+    | Skel.TBool => Int :: nil
+    | Skel.TZ => Int :: nil
+    | Skel.TTup t1 t2 => (ctyps_of_typ t1 ++ ctyps_of_typ t2)%list
     end.
   
+  Fixpoint nat_of_member {GS : list Skel.Typ} {ty : Skel.Typ}  (mem : member ty GS) : nat :=
+    match mem with
+    | HFirst _ => 0
+    | HNext _ _ m => S (nat_of_member m)
+    end.
+
+  Definition get_env {T : Type} {GS : list Skel.Typ} {ty : Skel.Typ}
+             (env : list T) (mem : member ty GS) (d : T) : T :=
+    List.nth (nat_of_member mem) env d.
+
+  Definition get_env_opt {T : Type} {GS : list Skel.Typ} {ty : Skel.Typ}
+             (env : list T) (mem : member ty GS) (d : T) : option T :=
+    nth_error env (nat_of_member mem).
+
   (* compiler of scalar expressions *)
-  Fixpoint compile_sexp (se : Sx.SExp) (env : SVEnv) : M (cmd * list exp) := match se with
-    | Sx.EVar v _ => ret (Cskip, S.vars2es (env v))
-    | Sx.ENum z => ret (Cskip, Enum z :: nil)
-    | Sx.ELet x e1 e2 _ =>
+  Fixpoint compile_sexp {GA GS : list Skel.Typ} {typ : Skel.Typ}
+           (se : Skel.SExp GA GS typ) (env : list (list var)) : M (cmd * list exp) := match se with
+    | Skel.EVar _ _ _ v => ret (Cskip, S.vars2es (get_env env v nil))
+    | Skel.ENum _ _ z => ret (Cskip, Enum z :: nil)
+    | Skel.ELet _ _ t1 t2 e1 e2 =>
       compile_sexp e1 env >>= fun ces1 => 
       let (c1, es1) := ces1 in
       (* let dim := length es1 in *)
-      let dim := ctyps_of_typ (Sx.typ_of_sexp e1) in
+      let dim := ctyps_of_typ t1 in
       freshes (length dim) >>= fun xs =>
-      compile_sexp e2 (upd env x xs) >>= fun ces2 => 
+      compile_sexp e2 (xs :: env) >>= fun ces2 => 
       let (c2, es2) := ces2 in
       ret (c1 ;; S.read_tup xs dim es1 ;; c2, es2)
-    | Sx.EBin op e1 e2 _ => 
+    | Skel.EBin _ _ _ _ _ op e1 e2 => 
       compile_sexp e1 env >>= fun ces1 =>
       let (c1, es1) := ces1 in
       compile_sexp e2 env >>= fun ces2 =>
@@ -172,47 +185,39 @@ Section compiler.
         ret (c1;; c2;; c, es)
       | _, _ => fail ""
       end
-    | Sx.EA va e _ =>
-      let dim := ctyps_of_typ (Sx.typ_of_sexp se) in
+    | Skel.EA _ _ typ va e =>
+      let dim := ctyps_of_typ typ in
       compile_sexp e env >>= fun ces =>
       let (c, es) := ces in
-      let (_, aname) := avarenv va in
+      let (_, aname) := get_env avarenv va (Var "", nil) in
       freshes (length dim) >>= fun xs =>
       match es with
       | i :: nil => ret (c ;; S.gen_read Gl xs dim (S.vars2es aname) i, S.vars2es xs)
       | _ => fail ""
       end
-    | Sx.ELen xa =>
-      let (l, _) := avarenv xa in ret (Cskip, (Evar l) :: nil)
-    | Sx.EPrj e i ty =>
-      match Sx.typ_of_sexp e with
-      | Sx.TBool | Sx.TZ => fail ""
-      | Sx.TTup tys => 
-        let off := len_until_i tys i in
-        let l := len_at_i tys i in
-        compile_sexp e env >>= fun ces =>
-        let (c, es) := ces in
-        if le_dec (off + l) (len_of_ty (Sx.TTup tys)) then
-          ret (c, firstn l (skipn off es))
-        else (* fail ("overflow the index " ++ S.nat_to_string i ++ " of tuple:" ++ "type of tuple: " ++ string_of_ty ty ++ *)
-             (*       "expected length = " ++ S.nat_to_string (len_of_ty ty) ++ *)
-             (*       "actual length = " ++ S.nat_to_string off ++ " + " ++ S.nat_to_string l) *)
-             fail ""
-      end
-    | Sx.ECons es _ => 
-      let fix compile_sexps (es : list Sx.SExp) env : M (cmd * list exp) :=
-          match es with
-          | nil => ret (Cskip, nil)
-          | (e :: es)%list =>
-            compile_sexp e env >>= fun ces =>
-            let (c, ge) := ces in
-            compile_sexps es env >>= fun ces' =>
-            let (c', ges) := ces' in
-            ret (c ;; c', ge ++ ges)
-          end in
-      compile_sexps es env
-    | Sx.EIf e1 e2 e3 _ =>
-      let dim := ctyps_of_typ (Sx.typ_of_sexp se) in
+    | Skel.ELen _ _ _ xa =>
+      let (l, _) := get_env avarenv xa (Var "", nil) in ret (Cskip, (Evar l) :: nil)
+    | Skel.EPrj1 _ _ t1 t2 e =>
+      let off := 0 in
+      let l := len_of_ty t1 in
+      compile_sexp e env >>= fun ces =>
+      let (c, es) := ces in
+      ret (c, firstn l (skipn off es))
+    | Skel.EPrj2 _ _ t1 t2 e =>
+      let off := len_of_ty t1 in
+      let l := len_of_ty t2 in
+      (* ugly copy and paste !*)
+      compile_sexp e env >>= fun ces =>
+      let (c, es) := ces in
+      ret (c, firstn l (skipn off es))
+    | Skel.ECons _ _ t1 t2 e1 e2 => 
+      compile_sexp e1 env >>= fun ces =>
+      let (c1, ge1) := ces in
+      compile_sexp e2 env >>= fun ces =>
+      let (c2, ge2) := ces in
+      ret (c1 ;; c2, ge1 ++ ge2)
+    | Skel.EIf _ _ ty e1 e2 e3 =>
+      let dim := ctyps_of_typ ty in
       compile_sexp e1 env >>= fun ces1 => 
       let (c1, e1) := ces1 in
       compile_sexp e2 env >>= fun ces2 =>
@@ -229,30 +234,26 @@ Section compiler.
 End compiler.
 
 Section TestCompiler.
-  Import Sx.
-  Definition EVar' (x : varE) := EVar x TZ.
-  Definition ELet' (x : varE) (e e' : SExp)  := ELet x e e' TZ.
-  Definition EBin' (op : SOp) (e1 e2 : SExp) := EBin op e1 e2 TZ.
-  Definition EA' (x : varA) (e : SExp) (typ : Typ) := EA x e TZ.
-  Definition EPrj' (e : SExp) (i : nat) := EPrj e i TZ.
-  Definition ECons' (es : list SExp) := ECons es TZ.
-  Definition EIf' (e e' e'' : SExp) := EIf e e' e'' TZ.
+  Import Skel.
+  Arguments EVar {GA GS t} _.
+  Arguments ELet {GA GS t1 t2} _ _.
+  Arguments EBin {GA GS t1 t2 t3} _ _ _.
+  Arguments EA {GA GS t} _ _.
+  Arguments EPrj1 {GA GS t1 t2} _.
+  Arguments EPrj2 {GA GS t1 t2} _.
+  Arguments ECons {GA GS t1 t2} _ _.
+  Arguments EIf {GA GS t} _ _ _.
+  Arguments ENum {GA GS} _.
   
   Open Scope string_scope.
 
-  Coercion VarE : string >-> varE.
-  Coercion ENum : Z >-> SExp.
-  Coercion EVar' : varE >-> SExp.
-
-  Definition test1 :=
-    typing emp_opt emp_opt(
-             ELet' "x" (ECons' ((1%Z : SExp)  :: (2%Z : SExp) :: nil)) (
-                     ELet' "y" (ECons' ((3%Z : SExp)  :: (4%Z : SExp) :: nil)) (
-                             ELet' "z" (ECons' (("x" : SExp) :: ("y" : SExp) :: nil)) ( 
-                                     EPrj' "z" 0)))).
+  Definition test1 : Skel.SExp nil nil (TTup TZ TZ) :=
+    ELet (ECons (ENum 1%Z) (ENum 2%Z)) (
+    ELet (ECons (ENum 3%Z) (ENum 4%Z)) (
+    ELet (ECons (EVar HFirst) (EVar (HNext HFirst))) (
+    EPrj1 (EVar HFirst)))).
   
-  Eval cbv in test1.
-  Eval cbv in (match test1 with Some (t, _) => Some (compile_sexp (emp_def (Var "error", nil)) t (emp_def nil) 0) | None => None end).
+  Eval cbv in (compile_sexp nil test1 nil 0).
   
 End TestCompiler.
 
@@ -260,101 +261,101 @@ Require Import pmap_skel.
 Require Import Reduce_opt_skel.
 Import Skel_lemma scan_lib.
 
-Module VarE_eq : DecType with Definition t := varE with Definition eq_dec := eq_dec.
-  Definition t := varE.
-  Definition eq (x y : t) := x = y.
-  Definition eq_equiv : Equivalence eq.
-  Proof.
-    split; cbv; intros; congruence.
-  Qed.
-  Definition eq_dec := eq_dec.
-End VarE_eq.
+(* Module VarE_eq : DecType with Definition t := varE with Definition eq_dec := eq_dec. *)
+(*   Definition t := varE. *)
+(*   Definition eq (x y : t) := x = y. *)
+(*   Definition eq_equiv : Equivalence eq. *)
+(*   Proof. *)
+(*     split; cbv; intros; congruence. *)
+(*   Qed. *)
+(*   Definition eq_dec := eq_dec. *)
+(* End VarE_eq. *)
 
-Module VarA_eq : DecType with Definition t := varA with Definition eq_dec := @eq_dec varA _.
-  Definition t := varA.
-  Definition eq (x y : t) := x = y.
-  Definition eq_equiv : Equivalence eq.
-  Proof.
-    split; cbv; intros; congruence. 
-  Qed.
-  Definition eq_dec := @eq_dec t _.
-End VarA_eq.
+(* Module VarA_eq : DecType with Definition t := varA with Definition eq_dec := @eq_dec varA _. *)
+(*   Definition t := varA. *)
+(*   Definition eq (x y : t) := x = y. *)
+(*   Definition eq_equiv : Equivalence eq. *)
+(*   Proof. *)
+(*     split; cbv; intros; congruence.  *)
+(*   Qed. *)
+(*   Definition eq_dec := @eq_dec t _. *)
+(* End VarA_eq. *)
 
-Instance eq_type_pair A B `{eq_type A} `{eq_type B} : eq_type (A * B) := {
-  eq_dec := _
-}.
-Proof.
-  intros; destruct H, H0; repeat decide equality.
-Qed.
+(* Instance eq_type_pair A B `{eq_type A} `{eq_type B} : eq_type (A * B) := { *)
+(*   eq_dec := _ *)
+(* }. *)
+(* Proof. *)
+(*   intros; destruct H, H0; repeat decide equality. *)
+(* Qed. *)
 
-Instance eq_type_STyp : eq_type Sx.Typ := {
-  eq_dec := Sx.STyp_eq_dec
-}.
+(* Instance eq_type_STyp : eq_type Sx.Typ := { *)
+(*   eq_dec := Sx.STyp_eq_dec *)
+(* }. *)
 
-Module VarATy_eq : DecType with Definition t := (varA * Sx.Typ)%type with Definition eq_dec := @eq_dec (varA * Sx.Typ) _.
-  Definition t := (varA * Sx.Typ)%type.
-  Definition eq (x y : t) := x = y.
-  Definition eq_equiv : Equivalence eq.
-  Proof.
-    split; cbv; intros; congruence. 
-  Qed.
-  Definition eq_dec := @eq_dec t _.
-End VarATy_eq.
+(* Module VarATy_eq : DecType with Definition t := (varA * Sx.Typ)%type with Definition eq_dec := @eq_dec (varA * Sx.Typ) _. *)
+(*   Definition t := (varA * Sx.Typ)%type. *)
+(*   Definition eq (x y : t) := x = y. *)
+(*   Definition eq_equiv : Equivalence eq. *)
+(*   Proof. *)
+(*     split; cbv; intros; congruence.  *)
+(*   Qed. *)
+(*   Definition eq_dec := @eq_dec t _. *)
+(* End VarATy_eq. *)
 
-Module SA := MSets VarA_eq.
-Module SATy := MSets VarATy_eq.
-Module SE := MSets VarE_eq.
+(* Module SA := MSets VarA_eq. *)
+(* Module SATy := MSets VarATy_eq. *)
+(* Module SE := MSets VarE_eq. *)
 
 Require Import Host.
 (* Instance CUDA_monad : Monad CUDA := {| ret := @ret; bind := bind |}. *)
 
 Section Compiler.
-  Fixpoint free_sv (e : Sx.SExp) : SE.t :=
-    match e with
-    | Sx.EVar v _ => SE.singleton v
-    | Sx.ENum _   => SE.empty
-    | Sx.ELet x e1 e2 _ => 
-      SE.union (free_sv e1) (SE.remove x (free_sv e2))
-    | Sx.EBin _ e1 e2 _ => SE.union (free_sv e1) (free_sv e2)
-    | Sx.EA _ e _ => free_sv e
-    | Sx.ELen _ => SE.empty
-    | Sx.EPrj e _ _ => free_sv e
-    | Sx.ECons es _ => fold_right (fun e xs => SE.union (free_sv e) xs) SE.empty es
-    | Sx.EIf e e' e'' _ => SE.union (free_sv e) (SE.union (free_sv e') (free_sv e''))
-    end.
+  (* Fixpoint free_sv (e : Sx.SExp) : SE.t := *)
+  (*   match e with *)
+  (*   | Sx.EVar v _ => SE.singleton v *)
+  (*   | Sx.ENum _   => SE.empty *)
+  (*   | Sx.ELet x e1 e2 _ =>  *)
+  (*     SE.union (free_sv e1) (SE.remove x (free_sv e2)) *)
+  (*   | Sx.EBin _ e1 e2 _ => SE.union (free_sv e1) (free_sv e2) *)
+  (*   | Sx.EA _ e _ => free_sv e *)
+  (*   | Sx.ELen _ => SE.empty *)
+  (*   | Sx.EPrj e _ _ => free_sv e *)
+  (*   | Sx.ECons es _ => fold_right (fun e xs => SE.union (free_sv e) xs) SE.empty es *)
+  (*   | Sx.EIf e e' e'' _ => SE.union (free_sv e) (SE.union (free_sv e') (free_sv e'')) *)
+  (*   end. *)
 
-  Fixpoint free_av (e : Sx.SExp) : SA.t :=
-    match e with
-    | Sx.EVar v _ => SA.empty
-    | Sx.ENum _   => SA.empty
-    | Sx.ELet x e1 e2 _ => 
-      SA.union (free_av e1) (free_av e2)
-    | Sx.EBin _ e1 e2 _ => SA.union (free_av e1) (free_av e2)
-    | Sx.EA x e _ => SA.add x (free_av e)
-    | Sx.ELen x => SA.singleton x
-    | Sx.EPrj e _ _ => free_av e
-    | Sx.ECons es _ => fold_right (fun e xs => SA.union (free_av e) xs) SA.empty es
-    | Sx.EIf e e' e'' _ => SA.union (free_av e) (SA.union (free_av e') (free_av e''))
-    end.
+  (* Fixpoint free_av (e : Sx.SExp) : SA.t := *)
+  (*   match e with *)
+  (*   | Sx.EVar v _ => SA.empty *)
+  (*   | Sx.ENum _   => SA.empty *)
+  (*   | Sx.ELet x e1 e2 _ =>  *)
+  (*     SA.union (free_av e1) (free_av e2) *)
+  (*   | Sx.EBin _ e1 e2 _ => SA.union (free_av e1) (free_av e2) *)
+  (*   | Sx.EA x e _ => SA.add x (free_av e) *)
+  (*   | Sx.ELen x => SA.singleton x *)
+  (*   | Sx.EPrj e _ _ => free_av e *)
+  (*   | Sx.ECons es _ => fold_right (fun e xs => SA.union (free_av e) xs) SA.empty es *)
+  (*   | Sx.EIf e e' e'' _ => SA.union (free_av e) (SA.union (free_av e') (free_av e'')) *)
+  (*   end. *)
 
-  Definition free_av_func (f : Sx.Func) :=
-    match f with
-    | Sx.F ps body => free_av body
-    end.
+  (* Definition free_av_func (f : Sx.Func) := *)
+  (*   match f with *)
+  (*   | Sx.F ps body => free_av body *)
+  (*   end. *)
 
-  Fixpoint free_av_lexp (e : Sx.LExp) : SA.t :=
-    match e with
-    | Sx.LNum _   => SA.empty
-    (* | Sx.LBin _ e1 e2 => SA.union (free_av_lexp e1) (free_av_lexp e2) *)
-    | Sx.LLen x => SA.singleton x 
-    end.
+  (* Fixpoint free_av_lexp (e : Sx.LExp) : SA.t := *)
+  (*   match e with *)
+  (*   | Sx.LNum _   => SA.empty *)
+  (*   (* | Sx.LBin _ e1 e2 => SA.union (free_av_lexp e1) (free_av_lexp e2) *) *)
+  (*   | Sx.LLen x => SA.singleton x  *)
+  (*   end. *)
 
-  Definition free_av_AE (ae : Sx.AE) :=
-    match ae with
-    | Sx.DArr f len =>
-      SA.union (free_av_func f) (free_av_lexp len)
-    | Sx.VArr xa => SA.singleton xa
-    end.
+  (* Definition free_av_AE (ae : Sx.AE) := *)
+  (*   match ae with *)
+  (*   | Sx.DArr f len => *)
+  (*     SA.union (free_av_func f) (free_av_lexp len) *)
+  (*   | Sx.VArr xa => SA.singleton xa *)
+  (*   end. *)
 
   Fixpoint map_opt {A B : Type} (f : A -> option B) (xs : list A) : option (list B) :=
     sequence (map f xs).
@@ -365,10 +366,10 @@ Section Compiler.
     | None => d
     end.
 
-  Definition idxEnv_of_sa (xas : SA.t) : Env varA nat _ :=
-    snd (SA.fold (fun xa (n_aenv : nat * Env varA nat _)  =>
-               let (n, aenv) := n_aenv in
-               (n + 1, upd aenv xa n)) xas (0, emp_def 0)).
+  (* Definition idxEnv_of_sa (xas : SA.t) : Env varA nat _ := *)
+  (*   snd (SA.fold (fun xa (n_aenv : nat * Env varA nat _)  => *)
+  (*              let (n, aenv) := n_aenv in *)
+  (*              (n + 1, upd aenv xa n)) xas (0, emp_def 0)). *)
 
   Definition arr_name n (d : list CTyp) :=
     List.combine
@@ -381,12 +382,12 @@ Section Compiler.
       (map Ptr d).
   Definition out_len_name := Var (name_of_len "Out").
 
-  Definition env_of_sa (aty_env : Env varA (option Sx.Typ) _)  (xas : SA.t) :
-    (Env varA (var * list (var * CTyp)) _) :=
-    let idxEnv := idxEnv_of_sa xas in
-    fun xa =>
-      let ctys := (ctyps_of_typ (opt_def (aty_env xa) Sx.TZ)) in
-      (len_name (idxEnv xa), arr_name (idxEnv xa) ctys).
+  (* Definition env_of_sa (aty_env : Env varA (option Sx.Typ) _)  (xas : SA.t) : *)
+  (*   (Env varA (var * list (var * CTyp)) _) := *)
+  (*   let idxEnv := idxEnv_of_sa xas in *)
+  (*   fun xa => *)
+  (*     let ctys := (ctyps_of_typ (opt_def (aty_env xa) Sx.TZ)) in *)
+  (*     (len_name (idxEnv xa), arr_name (idxEnv xa) ctys). *)
 
   Definition zipWith {A B C : Type} (f : A -> B -> C) (xs : list A) (ys : list B) :=
     map (fun xy => f (fst xy) (snd xy)) (combine xs ys).
@@ -409,63 +410,48 @@ Section Compiler.
     | S n => fun y => dumy_fun_n n x
     end.
 
-  Fixpoint compile_func_n' n (xs : list (varE * Sx.Typ)) svar_env avar_env body :=
-    match n return type_of_func n with
-    | O =>
-      match xs with
-      | nil => evalM (compile_sexp avar_env body svar_env) 0 (Cskip, nil)
-      | _ :: _ => (Cskip, nil)
-      end
-    | S n =>
-      match xs with
-      | nil => dumy_fun_n (S n) (Cskip, nil)
-      | (x, _) :: xs =>
-        fun x' =>
-          compile_func_n' n xs (upd svar_env x x') avar_env body
-      end
+  Definition type_of_ftyp (fty : Skel.FTyp) :=
+    match fty with
+    | Skel.Fun1 dom cod => list var -> (cmd * list exp)
+    | Skel.Fun2 dom1 dom2 cod  => list var -> list var -> (cmd * list exp)
     end.
 
-  Definition compile_func_n n avar_env f :=
-    match f with
-    | Sx.F ps body => compile_func_n' n ps (emp_def nil) avar_env body
+  Fixpoint compile_func {GA fty} avar_env (body : Skel.Func GA fty) :=
+    match body in Skel.Func _ fty' return type_of_ftyp fty' with
+    | Skel.F1 _ _ _ body => fun xs => evalM (compile_sexp avar_env body (xs :: nil)) 0 (Cskip, nil)
+    | Skel.F2 _ _ _ _ body => fun xs ys => evalM (compile_sexp avar_env body (xs :: ys :: nil)) 0 (Cskip, nil)
     end.
 
-  Definition compile_lexp (aenv : Env varA (hostVar * list hostVar) _) le : expr :=
+  Definition compile_lexp {GA ty} (aenv : list (hostVar * list hostVar)) (le : Skel.LExp GA ty) : expr :=
     match le with
-    | Sx.LNum n => Const n
-    | Sx.LLen a => VarE (fst (aenv a))
+    | Skel.LNum _ n => Const n
+    | Skel.LLen _ _ a => VarE (fst (get_env aenv a (0, nil)))
     end.
 
-  Definition accessor_of_array aenv arr tyxa :=
-    let i := SimplSkel.VarE "i" in
-    compile_func_n 1 aenv (Sx.F ((i, Sx.TZ) :: nil)
-                                (Sx.EA arr (Sx.EVar i Sx.TZ) tyxa)).
+  Definition accessor_of_array {GA tyxa} aenv (arr : member tyxa GA) :=
+    compile_func aenv (Skel.F1 _ Skel.TZ _ (Skel.EA _ _ _ arr (Skel.EVar _ _ _ HFirst))).
 
-  Definition compile_AE (aty_env : Env varA (option Sx.Typ) _)
-             avar_env (var_ptr_env : Env varA (hostVar * list hostVar) _) ae :
+  Definition compile_AE {GA ty}
+             avar_env (var_ptr_env : list (hostVar * list hostVar)) (ae : Skel.AE GA ty) :
     ((var -> (cmd * list exp)) * expr) :=
     match ae with
-    | Sx.DArr f len =>
-      let f' := compile_func_n 1 avar_env f in
+    | Skel.DArr _ _ f len =>
+      let f' := compile_func avar_env f in
       let len' := compile_lexp var_ptr_env len in
       (fun x => f' (x :: nil), len')
-    | Sx.VArr xa =>
-      let tyxa := match aty_env xa with
-                  | None => Sx.TZ
-                  | Some tyxa => tyxa 
-                  end in
-      let get := accessor_of_array avar_env xa tyxa in
-      (fun x => get (x :: nil), VarE (fst (var_ptr_env xa)))
+    | Skel.VArr _ _ xa =>
+      let get := accessor_of_array avar_env xa in
+      (fun x => get (x :: nil), VarE (fst (get_env var_ptr_env xa (0, nil))))
     end.
 
   Variable ntrd : nat.
   Variable nblk : nat.
 
-  Definition Z_of_val (v : SVal) :=
-    match v with
-    | VB _ | VTup _ => 0%Z
-    | VZ n => n
-    end.
+  (* Definition Z_of_val (v : SVal) := *)
+  (*   match v with *)
+  (*   | VB _ | VTup _ => 0%Z *)
+  (*   | VZ n => n *)
+  (*   end. *)
   
   Open Scope string_scope.
 
@@ -475,14 +461,14 @@ Section Compiler.
     | xs :: xss => (xs ++ concat xss)%list
     end.
 
-  Definition shiftn n (var_host_env : Env varA (hostVar * list hostVar) _) :=
-    env_map (fun xs => (n + (fst xs), List.map (fun x => n + x) (snd xs))) var_host_env.
+  (* Definition shiftn n (var_host_env : list (hostVar * list hostVar)) := *)
+  (*   map (fun xs => (n + (fst xs), List.map (fun x => n + x) (snd xs))) var_host_env. *)
 
   Instance eq_kerID : eq_type kerID := {
     eq_dec := Nat.eq_dec
   }.
 
-  Eval compute in accessor_of_array (emp_def (Var "len", Var "a" :: nil)) (VarA "a") Sx.TZ (Var "i" :: nil).
+  (* Eval compute in accessor_of_array (emp_def (Var "len", Var "a" :: nil)) (VarA "a") Sx.TZ (Var "i" :: nil). *)
 
   Fixpoint alloc_tup_arr v n len :=
     match n with
@@ -490,14 +476,69 @@ Section Compiler.
     | S n => alloc v len :: alloc_tup_arr (S v) n len
     end.
 
+  Variable sorry : forall {T : Type}, T.
+  Arguments sorry {T}.
+
+  Definition state s a := s -> (a * s).
+  Instance state_Monad s : Monad (state s) := {
+     ret A x := fun n => (x, n);
+     bind A B x f := fun n => let (y, n) := x n in f y n
+  }.
+  Definition getS {s} : state s s := fun x => (x, x).
+  Definition setS {s} x : state s unit := fun _ => (tt, x).
+
+  Open Scope list_scope.
+
+  Definition fLet e : state (nat * list instr) hostVar :=
+    do! st := getS in
+    let (n, irs) := st : nat * list instr in
+    do! _ := setS (S n, irs ++ (iLet n e :: nil)) in
+    ret n.
+
+  Definition fAlloc e : state (nat * list instr) hostVar :=
+    do! st := getS in
+    let (n, irs) := st : nat * list instr in
+    do! _ := setS (S n, irs ++ (alloc n e :: nil)) in
+    ret n.
+
+  Definition fAllocs ctys e : state (nat * list instr) (list hostVar) :=
+    mapM (fun cty => fAlloc e) ctys.
+
+  Definition gen_params (GA : list Skel.Typ) : list (var * list var) :=
+    let f typ i :=
+        let ctyp := ctyps_of_typ typ in
+    zipWith (fun p  => 
+      let (typ, i) := p in ) (GA (seq 0 (length GA)))
+
+  Definition compile_Skel {GA typ} (host_var_env : list (hostVar * list hostVar))
+             (skel : Skel.SkelE GA typ) : Host.Prog * nat :=
+    match skel with
+    | Skel.Map _ dom cod f arr =>
+      let (g, outlen) := compile_AE _ host_var_env arr in
+      do! outlenVar := fLet outLen in
+      
+    | Skel.Reduce _ typ f arr => sorry
+    | Skel.Seq _ start len => sorry
+    | Skel.Zip _ typ1 typ2 arr1 arr2 => sorry
+    end.
+
+  Fixpoint compile_AS {GA typ} (numVar : nat) (host_var_env : list (hostVar * list hostVar)) (p : Skel.AS GA typ) : Host.Prog :=
+    match p with
+    | Skel.ALet _ tskel tyres skel res => 
+      let '((instrs, outs, kers), n) := compile_Skel host_var_env skel in
+      let '(instrs_res, outs_res, kers_res) := compile_AS n (outs :: host_var_env) res in
+      (instrs ++ instrs_res, outs_res, kers ++ kers_res)
+    | Skel.ARet _ _ x =>
+      (nil, get_env host_var_env x (0, nil), nil)
+    end%list.
+
   Fixpoint compile_AS
            (numVar : nat)
            (aty_env : Env varA (option Sx.Typ) _)
            (host_var_env : Env varA (hostVar * list hostVar) _)
            (p : Sx.AS) : Host.Prog :=
     match p with
-    | Sx.ALet xa tyxa
-              {| Sx.skel_name := skl; Sx.skel_fs := fs; Sx.skel_aes := aes; Sx.skel_les := se |} rest =>
+    | Sx.ALet xa tyxa skelE rest =>
       let fvs_f := List.fold_right (fun f sa => SA.union (free_av_func f) sa) SA.empty fs in
       let fvs_ae := List.fold_right (fun ae sa => SA.union (free_av_AE (fst ae)) sa) SA.empty aes in
       let fvs := SA.union fvs_f fvs_ae in
@@ -522,8 +563,8 @@ Section Compiler.
 
       let env' := env_map (fun x => (fst x, List.map fst (snd x))) env in
 
-      match skl, fs, aes with 
-     | "map", (f :: nil), ((ae, tyAe) :: nil) =>
+      match skelE with 
+     | SkelMap f (ae, tyAe) =>
         (* the dimension of the input array *)
         let inDim := ctyps_of_typ tyAe in
         let (get, inlen) := compile_AE aty_env env' host_var_env ae in
